ecoop17/dot_storeless_wfrel_aux.v
@@ -460,3 +460,63 @@ Proof.
       optFuncs_det;
       eauto.
 Qed.
+
+Definition venv := list dms.
+Definition tenv := list ty.
+Hint Unfold venv.
+Hint Unfold tenv.
+
+Inductive R_env (k : nat) : venv -> tenv -> Set :=
+| R_nil :
+    R_env k [] []
+| R_cons : forall T v env G,
+    R_env k env G ->
+    vtp (open 0 (VObj v) T) k (tvar (VObj v)) ->
+    R_env k (v :: env) (T :: G)
+.
+Hint Constructors R_env.
+
+Lemma R_env_mon: forall G env m n,
+    R_env n env G ->
+    m <= n ->
+    R_env m env G.
+Proof. intros * Henv; induction Henv; eauto. Qed.
+Hint Resolve R_env_mon.
+
+Lemma wf_length : forall k vs ts,
+                    R_env k vs ts ->
+                    (length vs = length ts).
+Proof. intros * H; induction H; simpl; congruence. Qed.
+Hint Resolve wf_length.
+
+Ltac lenG_to_lenEnv :=
+  try match goal with
+  | H: R_env _ ?env ?G |- _ =>
+    replace (length G) with (length env) in * by (eauto using wf_length)
+  end.
+
+Hint Constructors Forall.
+
+Ltac inverts_if_nonvar x H :=
+    tryif is_var x then fail else inverts H.
+Ltac inverts_closed :=
+  match goal with
+  | H : vr_closed _ _ ?v  |- _ =>
+    inverts_if_nonvar v H
+  | H : closed _ _ ?T     |- _ =>
+    inverts_if_nonvar T H
+  | H : tm_closed _ _ ?t  |- _ =>
+    inverts_if_nonvar t H
+  | H : dm_closed _ _ ?d  |- _ =>
+    inverts_if_nonvar d H
+  | H : dms_closed _ _ ?d |- _ =>
+    inverts_if_nonvar d H
+  end.
+
+Lemma env_dms_closed: forall k env G l, R_env k env G -> length env = l -> Forall (dms_closed 0 1) env.
+Proof.
+  induction env; intros * Henv Hl; subst; inverts Henv; constructor; simpl; eauto using Forall_impl.
+  assert (tm_closed 0 0 (tvar (VObj a))) by (eauto using vtp_v_closed); repeat inverts_closed; eauto.
+Qed.
+
+Hint Resolve env_dms_closed.
